examples/formal-languages/context-free/locationScript.sml
@@ -33,7 +33,34 @@ val map_loc_def = Define`
                              <| row := n; col := 1; offset := 0 |>)) ::
                         map_loc t (n+1))     `;
 
+
+val merge_locs_assoc = Q.store_thm(
+  "merge_locs_assoc[simp]",
+  ‘(merge_locs (merge_locs l1 l2) l3 = merge_locs l1 l3) ∧
+   (merge_locs l1 (merge_locs l2 l3) = merge_locs l1 l3)’,
+  map_every Cases_on [`l1`, `l2`, `l3`] >>
+  simp[merge_locs_def]);
+
+val merge_list_locs_2 = Q.store_thm(
+  "merge_list_locs_2[simp]",
+  ‘∀h1 h2 t.
+     merge_list_locs (h1 :: h2 :: t) = merge_list_locs (merge_locs h1 h2 :: t)’,
+  Induct_on ‘t’ >> simp[merge_list_locs_def]);
+
+val merge_list_locs_nested = Q.store_thm(
+  "merge_list_locs_nested[simp]",
+  ‘∀h t1 t2. merge_list_locs (merge_list_locs (h::t1) :: t2) =
+             merge_list_locs (h :: t1 ++ t2)’,
+  Induct_on ‘t1’ >> simp[merge_list_locs_def]);
+
+val merge_list_locs_sing = Q.store_thm(
+  "merge_list_locs_sing[simp]",
+  ‘merge_list_locs [h] = h’,
+  simp[merge_list_locs_def]);
+
+val merge_locs_idem = Q.store_thm(
+  "merge_locs_idem[simp]",
+  ‘merge_locs l l = l’,
+  Cases_on ‘l’ >> simp[merge_locs_def]);
+
 val _ = export_theory();
-
-
-
